<?xml version="1.0"?>
<rdf:RDF xmlns="http://emmo.info/perspectives/emmo-semiotics.owl#"
     xml:base="http://emmo.info/perspectives/emmo-semiotics.owl"
     xmlns:owl="http://www.w3.org/2002/07/owl#"
     xmlns:rdf="http://www.w3.org/1999/02/22-rdf-syntax-ns#"
     xmlns:xml="http://www.w3.org/XML/1998/namespace"
     xmlns:xsd="http://www.w3.org/2001/XMLSchema#"
     xmlns:rdfs="http://www.w3.org/2000/01/rdf-schema#"
     xmlns:emmo-annotations="http://emmo.info/base/emmo-annotations.owl#">
    <owl:Ontology rdf:about="http://emmo.info/perspectives/emmo-semiotics.owl">
        <owl:imports rdf:resource="http://emmo.info/perspectives/emmo-processual.owl"/>
        <emmo-annotations:EMMO_5525a055_dda5_4556_8b91_f0d22fa676cc>EMMO is released under a Creative Commons license Attribution 4.0 International (CC BY 4.0)

https://creativecommons.org/licenses/by/4.0/legalcode</emmo-annotations:EMMO_5525a055_dda5_4556_8b91_f0d22fa676cc>
        <emmo-annotations:EMMO_cd5fb112_7ee7_4120_a35d_3ca3e6c3f4ab>Emanuele Ghedini (University of Bologna, IT)
Gerhard Goldbeck (GCL Ltd, UK)
Adham Hashibon (Fraunhofer IWM, DE)
Georg Schmitz (Access, DE)
Jesper Friis (SINTEF, NO)</emmo-annotations:EMMO_cd5fb112_7ee7_4120_a35d_3ca3e6c3f4ab>
        <rdfs:comment>Contacts:
Gerhard Goldbeck
Goldbeck Consulting Ltd (UK)
email: gerhard@goldbeck-consulting.com

Emanuele Ghedini
University of Bologna (IT)
email: emanuele.ghedini@unibo.it</rdfs:comment>
        <rdfs:comment>European Materials and Modelling Ontology (EMMO)

EMMO is a multidisciplinary effort to develop a standard representational framework (the ontology) based on current materials modelling knowledge, including physical sciences, analytical philosophy and information and communication technologies. 

It provides the connection between the physical world, materials characterisation world and materials modelling world.</rdfs:comment>
        <rdfs:comment>The EMMO requires FacT++ reasoner plugin in order to visualize all inferences and class hierarchy (ctrl+R hotkey in Protege).</rdfs:comment>
        <owl:versionInfo>The European Materials Modelling Ontology

Version 0.9.10</owl:versionInfo>
    </owl:Ontology>
    


    <!-- 
    ///////////////////////////////////////////////////////////////////////////////////////
    //
    // Object Properties
    //
    ///////////////////////////////////////////////////////////////////////////////////////
     -->

    


    <!-- http://emmo.info/perspectives/emmo-semiotics.owl#EMMO_2337e25c_3c60_43fc_a8f9_b11a3f974291 -->

    <owl:ObjectProperty rdf:about="http://emmo.info/perspectives/emmo-semiotics.owl#EMMO_2337e25c_3c60_43fc_a8f9_b11a3f974291">
        <rdfs:subPropertyOf rdf:resource="http://emmo.info/base/emmo-mereotopology.owl#EMMO_ec2472ae_cf4a_46a5_8555_1556f5a6c3c5"/>
        <emmo-annotations:EMMO_967080e5_2f42_4eb2_a3a9_c58143e835f9>The generic EMMO semiotical relation.</emmo-annotations:EMMO_967080e5_2f42_4eb2_a3a9_c58143e835f9>
        <rdfs:label xml:lang="en">semiotical</rdfs:label>
    </owl:ObjectProperty>
    


    <!-- http://emmo.info/perspectives/emmo-semiotics.owl#EMMO_297999d6_c9e4_4262_9536_bd524d1c6e21 -->

    <owl:ObjectProperty rdf:about="http://emmo.info/perspectives/emmo-semiotics.owl#EMMO_297999d6_c9e4_4262_9536_bd524d1c6e21">
        <rdfs:subPropertyOf rdf:resource="http://emmo.info/perspectives/emmo-semiotics.owl#EMMO_60577dea_9019_4537_ac41_80b0fb563d41"/>
        <rdfs:range rdf:resource="http://emmo.info/perspectives/emmo-semiotics.owl#EMMO_0cd58641_824c_4851_907f_f4c3be76630c"/>
        <rdfs:label xml:lang="en">hasIndex</rdfs:label>
    </owl:ObjectProperty>
    


    <!-- http://emmo.info/perspectives/emmo-semiotics.owl#EMMO_39c3815d_8cae_4c8f_b2ff_eeba24bec455 -->

    <owl:ObjectProperty rdf:about="http://emmo.info/perspectives/emmo-semiotics.owl#EMMO_39c3815d_8cae_4c8f_b2ff_eeba24bec455">
        <rdfs:subPropertyOf rdf:resource="http://emmo.info/perspectives/emmo-semiotics.owl#EMMO_60577dea_9019_4537_ac41_80b0fb563d41"/>
        <rdfs:range rdf:resource="http://emmo.info/perspectives/emmo-semiotics.owl#EMMO_d7788d1a_020d_4c78_85a1_13563fcec168"/>
        <rdfs:label xml:lang="en">hasIcon</rdfs:label>
    </owl:ObjectProperty>
    


    <!-- http://emmo.info/perspectives/emmo-semiotics.owl#EMMO_60577dea_9019_4537_ac41_80b0fb563d41 -->

    <owl:ObjectProperty rdf:about="http://emmo.info/perspectives/emmo-semiotics.owl#EMMO_60577dea_9019_4537_ac41_80b0fb563d41">
        <rdfs:subPropertyOf rdf:resource="http://emmo.info/perspectives/emmo-semiotics.owl#EMMO_2337e25c_3c60_43fc_a8f9_b11a3f974291"/>
        <rdfs:domain rdf:resource="http://emmo.info/perspectives/emmo-semiotics.owl#EMMO_6f5af708_f825_4feb_a0d1_a8d813d3022b"/>
        <rdfs:range rdf:resource="http://emmo.info/perspectives/emmo-semiotics.owl#EMMO_b21a56ed_f969_4612_a6ec_cb7766f7f31d"/>
        <rdfs:label xml:lang="en">hasSign</rdfs:label>
    </owl:ObjectProperty>
    


    <!-- http://emmo.info/perspectives/emmo-semiotics.owl#EMMO_7fb7fe7e_bdf9_4eeb_adad_e384dd5285c6 -->

    <owl:ObjectProperty rdf:about="http://emmo.info/perspectives/emmo-semiotics.owl#EMMO_7fb7fe7e_bdf9_4eeb_adad_e384dd5285c6">
        <rdfs:subPropertyOf rdf:resource="http://emmo.info/perspectives/emmo-semiotics.owl#EMMO_60577dea_9019_4537_ac41_80b0fb563d41"/>
        <rdfs:range rdf:resource="http://emmo.info/perspectives/emmo-semiotics.owl#EMMO_054af807_85cd_4a13_8eba_119dfdaaf38b"/>
        <rdfs:label xml:lang="en">hasInterpretant</rdfs:label>
    </owl:ObjectProperty>
    


    <!-- http://emmo.info/perspectives/emmo-semiotics.owl#EMMO_eb3518bf_f799_4f9e_8c3e_ce59af11453b -->

    <owl:ObjectProperty rdf:about="http://emmo.info/perspectives/emmo-semiotics.owl#EMMO_eb3518bf_f799_4f9e_8c3e_ce59af11453b">
        <rdfs:subPropertyOf rdf:resource="http://emmo.info/perspectives/emmo-semiotics.owl#EMMO_60577dea_9019_4537_ac41_80b0fb563d41"/>
        <rdfs:range rdf:resource="http://emmo.info/perspectives/emmo-semiotics.owl#EMMO_35d2e130_6e01_41ed_94f7_00b333d46cf9"/>
        <rdfs:label xml:lang="en">hasConvention</rdfs:label>
    </owl:ObjectProperty>
    


    <!-- 
    ///////////////////////////////////////////////////////////////////////////////////////
    //
    // Classes
    //
    ///////////////////////////////////////////////////////////////////////////////////////
     -->

    


    <!-- http://emmo.info/perspectives/emmo-semiotics.owl#EMMO_008fd3b2_4013_451f_8827_52bceab11841 -->

    <owl:Class rdf:about="http://emmo.info/perspectives/emmo-semiotics.owl#EMMO_008fd3b2_4013_451f_8827_52bceab11841">
        <rdfs:subClassOf>
            <owl:Restriction>
                <owl:onProperty rdf:resource="http://emmo.info/perspectives/emmo-processual.owl#EMMO_ae2d1a96_bfa1_409a_a7d2_03d69e8a125a"/>
                <owl:someValuesFrom rdf:resource="http://emmo.info/perspectives/emmo-semiotics.owl#EMMO_0527413c_b286_4e9c_b2d0_03fb2a038dee"/>
            </owl:Restriction>
        </rdfs:subClassOf>
        <rdfs:subClassOf>
            <owl:Restriction>
                <owl:onProperty rdf:resource="http://emmo.info/perspectives/emmo-processual.owl#EMMO_c5aae418_1622_4d02_93c5_21159e28e6c1"/>
                <owl:someValuesFrom rdf:resource="http://emmo.info/perspectives/emmo-semiotics.owl#EMMO_6f5af708_f825_4feb_a0d1_a8d813d3022b"/>
            </owl:Restriction>
        </rdfs:subClassOf>
        <rdfs:subClassOf>
            <owl:Restriction>
                <owl:onProperty rdf:resource="http://emmo.info/perspectives/emmo-processual.owl#EMMO_c5aae418_1622_4d02_93c5_21159e28e6c1"/>
                <owl:someValuesFrom rdf:resource="http://emmo.info/perspectives/emmo-semiotics.owl#EMMO_b21a56ed_f969_4612_a6ec_cb7766f7f31d"/>
            </owl:Restriction>
        </rdfs:subClassOf>
        <emmo-annotations:EMMO_967080e5_2f42_4eb2_a3a9_c58143e835f9>A &apos;process&apos;, that has participant an &apos;interpreter&apos;, that is aimed to produce a &apos;sign&apos; representing another participant, the &apos;interpreted&apos;.</emmo-annotations:EMMO_967080e5_2f42_4eb2_a3a9_c58143e835f9>
        <emmo-annotations:EMMO_b432d2d5_25f4_4165_99c5_5935a7763c1a>Me looking a cat and saying loud: &quot;Cat!&quot; -&gt; the semiosis process

me -&gt; interpreter
cat -&gt; object (in Peirce semiotics)
the cat perceived by my mind -&gt; interpretant
&quot;Cat!&quot; -&gt; sign, the produced sign</emmo-annotations:EMMO_b432d2d5_25f4_4165_99c5_5935a7763c1a>
        <rdfs:label xml:lang="en">Semiosis</rdfs:label>
    </owl:Class>
    


    <!-- http://emmo.info/perspectives/emmo-semiotics.owl#EMMO_0527413c_b286_4e9c_b2d0_03fb2a038dee -->

    <owl:Class rdf:about="http://emmo.info/perspectives/emmo-semiotics.owl#EMMO_0527413c_b286_4e9c_b2d0_03fb2a038dee">
        <rdfs:subClassOf rdf:resource="http://emmo.info/perspectives/emmo-semiotics.owl#EMMO_b803f122_4acb_4064_9d71_c1e5fd091fc9"/>
        <rdfs:subClassOf>
            <owl:Restriction>
                <owl:onProperty rdf:resource="http://emmo.info/base/emmo-4d.owl#EMMO_f68030be_94b8_4c61_a161_886468558054"/>
                <owl:someValuesFrom rdf:resource="http://emmo.info/perspectives/emmo-semiotics.owl#EMMO_054af807_85cd_4a13_8eba_119dfdaaf38b"/>
            </owl:Restriction>
        </rdfs:subClassOf>
        <emmo-annotations:EMMO_967080e5_2f42_4eb2_a3a9_c58143e835f9>The entity (or agent, or observer, or cognitive entity) who connects &apos;sign&apos;, &apos;interpretant&apos; and &apos;object&apos;.</emmo-annotations:EMMO_967080e5_2f42_4eb2_a3a9_c58143e835f9>
        <rdfs:label xml:lang="en">Interpreter</rdfs:label>
    </owl:Class>
    


    <!-- http://emmo.info/perspectives/emmo-semiotics.owl#EMMO_054af807_85cd_4a13_8eba_119dfdaaf38b -->

    <owl:Class rdf:about="http://emmo.info/perspectives/emmo-semiotics.owl#EMMO_054af807_85cd_4a13_8eba_119dfdaaf38b">
        <rdfs:subClassOf rdf:resource="http://emmo.info/perspectives/emmo-semiotics.owl#EMMO_b21a56ed_f969_4612_a6ec_cb7766f7f31d"/>
        <rdfs:label xml:lang="en">Interpretant</rdfs:label>
    </owl:Class>
    


    <!-- http://emmo.info/perspectives/emmo-semiotics.owl#EMMO_0cd58641_824c_4851_907f_f4c3be76630c -->

    <owl:Class rdf:about="http://emmo.info/perspectives/emmo-semiotics.owl#EMMO_0cd58641_824c_4851_907f_f4c3be76630c">
        <emmo-annotations:EMMO_967080e5_2f42_4eb2_a3a9_c58143e835f9>A &apos;sign&apos; that stands for an &apos;objectì due to causal continguity.</emmo-annotations:EMMO_967080e5_2f42_4eb2_a3a9_c58143e835f9>
        <emmo-annotations:EMMO_b432d2d5_25f4_4165_99c5_5935a7763c1a>Smoke stands for a combustion process (a fire).

My facial expression stands for my emotional status.</emmo-annotations:EMMO_b432d2d5_25f4_4165_99c5_5935a7763c1a>
        <rdfs:label xml:lang="en">Index</rdfs:label>
    </owl:Class>
    


    <!-- http://emmo.info/perspectives/emmo-semiotics.owl#EMMO_35d2e130_6e01_41ed_94f7_00b333d46cf9 -->

    <owl:Class rdf:about="http://emmo.info/perspectives/emmo-semiotics.owl#EMMO_35d2e130_6e01_41ed_94f7_00b333d46cf9">
        <emmo-annotations:EMMO_967080e5_2f42_4eb2_a3a9_c58143e835f9>A &apos;sign&apos; that stand for an &apos;object&apos; through convention, norm or habit, without any resemblance to it.</emmo-annotations:EMMO_967080e5_2f42_4eb2_a3a9_c58143e835f9>
        <rdfs:label xml:lang="en">Conventional</rdfs:label>
    </owl:Class>
    


    <!-- http://emmo.info/perspectives/emmo-semiotics.owl#EMMO_6f5af708_f825_4feb_a0d1_a8d813d3022b -->

    <owl:Class rdf:about="http://emmo.info/perspectives/emmo-semiotics.owl#EMMO_6f5af708_f825_4feb_a0d1_a8d813d3022b">
        <owl:equivalentClass>
            <owl:Restriction>
                <owl:onProperty rdf:resource="http://emmo.info/perspectives/emmo-semiotics.owl#EMMO_60577dea_9019_4537_ac41_80b0fb563d41"/>
                <owl:someValuesFrom rdf:resource="http://emmo.info/perspectives/emmo-semiotics.owl#EMMO_b21a56ed_f969_4612_a6ec_cb7766f7f31d"/>
            </owl:Restriction>
        </owl:equivalentClass>
        <rdfs:subClassOf rdf:resource="http://emmo.info/perspectives/emmo-semiotics.owl#EMMO_b803f122_4acb_4064_9d71_c1e5fd091fc9"/>
        <emmo-annotations:EMMO_967080e5_2f42_4eb2_a3a9_c58143e835f9>The object, in Peirce semiotics.</emmo-annotations:EMMO_967080e5_2f42_4eb2_a3a9_c58143e835f9>
        <rdfs:comment>Here is assumed that the concept of &apos;object&apos; is always relative to a &apos;semiotic&apos; process. An &apos;object&apos; does not exists per se, but it&apos;s always part of an interpretation.

The EMMO relies on strong reductionism, i.e. everything real is a formless collection of elementary particles: we give a meaning to real world entities only by giving them boundaries and defining them using &apos;sign&apos;-s. 

In this way the &apos;sign&apos;-ed entity become and &apos;object&apos;, and the &apos;object&apos; is the basic entity needed in order to apply a logical formalism to the real world entities (i.e. we can speak of it through its sign, and use logics on it through its sign).</rdfs:comment>
        <rdfs:label xml:lang="en">Object</rdfs:label>
    </owl:Class>
    


    <!-- http://emmo.info/perspectives/emmo-semiotics.owl#EMMO_b21a56ed_f969_4612_a6ec_cb7766f7f31d -->

    <owl:Class rdf:about="http://emmo.info/perspectives/emmo-semiotics.owl#EMMO_b21a56ed_f969_4612_a6ec_cb7766f7f31d">
        <owl:equivalentClass>
            <owl:Class>
                <owl:unionOf rdf:parseType="Collection">
                    <rdf:Description rdf:about="http://emmo.info/perspectives/emmo-semiotics.owl#EMMO_0cd58641_824c_4851_907f_f4c3be76630c"/>
                    <rdf:Description rdf:about="http://emmo.info/perspectives/emmo-semiotics.owl#EMMO_35d2e130_6e01_41ed_94f7_00b333d46cf9"/>
                    <rdf:Description rdf:about="http://emmo.info/perspectives/emmo-semiotics.owl#EMMO_d7788d1a_020d_4c78_85a1_13563fcec168"/>
                </owl:unionOf>
            </owl:Class>
        </owl:equivalentClass>
        <rdfs:subClassOf rdf:resource="http://emmo.info/perspectives/emmo-semiotics.owl#EMMO_b803f122_4acb_4064_9d71_c1e5fd091fc9"/>
        <emmo-annotations:EMMO_967080e5_2f42_4eb2_a3a9_c58143e835f9>An &apos;spacetime&apos; that is used as sign (&quot;semeion&quot; in greek) that stands for another &apos;spacetime&apos; through an semiotic process.</emmo-annotations:EMMO_967080e5_2f42_4eb2_a3a9_c58143e835f9>
        <emmo-annotations:EMMO_b432d2d5_25f4_4165_99c5_5935a7763c1a>A novel is made of chapters, paragraphs, sentences, words and characters (in a direct parthood mereological hierarchy). 

Each of them are &apos;sign&apos;-s. 

A character can be the a-tomistic &apos;sign&apos; for the class of texts.

The horizontal segment in the character &quot;A&quot; is direct part of &quot;A&quot; but it is not a &apos;sign&apos; itself.

For plain text we can propose the ASCII symbols, for math the fundamental math symbols.</emmo-annotations:EMMO_b432d2d5_25f4_4165_99c5_5935a7763c1a>
        <rdfs:comment>A &apos;sign&apos; can have temporal-direct-parts which are &apos;sign&apos; themselves.

A &apos;sign&apos; usually have &apos;sign&apos; spatial direct parts only up to a certain elementary semiotic level, in which the part is only a &apos;physical&apos; and no more a &apos;sign&apos; (i.e. it stands for nothing). This elementary semiotic level is peculiar to each particular system of signs (e.g. text, painting).

Just like an &apos;elementary&apos; in the &apos;physical&apos; branch, each &apos;sign&apos; branch should have an a-tomistic mereological part.</rdfs:comment>
        <rdfs:comment>According to Peirce, &apos;sign&apos; includes three subcategories:
- symbols: that stand for an object through convention
- indeces: that stand for an object due to causal continguity
- icon: that stand for an object due to similitudes e.g. in shape or composition</rdfs:comment>
        <rdfs:comment>In a 4D ontology one could question if a &apos;sign&apos; should be defined as a spatial direct part of a &apos;semiosis&apos; i.e. a proper part of a &apos;semiosis&apos; during all its existence.

e.g. one can say that an unread text is not a &apos;sign&apos;: it was a &apos;sign&apos; during the &apos;semiosis&apos; process in which it was written, but after that it is something else, until somebody read it again.

However, this is not the case for an ontology, since declaring an individual under the &apos;sign&apos; class (a semiosis outside the EMMO, a meta-semiosis) is equivalent to say that for the ontologist (an interpreter outside the EMMO, a meta-interpreter) the real entity (an object outside the EMMO, a meta-object) is a &apos;sign&apos;.

So the &apos;semiosis&apos; process within the EMMO is about how other &apos;interpreter&apos;-s deal with the &apos;sign&apos;-s here declared.</rdfs:comment>
        <rdfs:comment>It can be defined as the semiotic branch of the EMMO.

&apos;sign&apos; subclasses categorize the type of signs that are used to create representations/models of the real world entities.</rdfs:comment>
        <rdfs:label xml:lang="en">Sign</rdfs:label>
    </owl:Class>
    


    <!-- http://emmo.info/perspectives/emmo-semiotics.owl#EMMO_b803f122_4acb_4064_9d71_c1e5fd091fc9 -->

    <owl:Class rdf:about="http://emmo.info/perspectives/emmo-semiotics.owl#EMMO_b803f122_4acb_4064_9d71_c1e5fd091fc9">
        <owl:equivalentClass>
            <owl:Class>
                <owl:unionOf rdf:parseType="Collection">
                    <rdf:Description rdf:about="http://emmo.info/perspectives/emmo-semiotics.owl#EMMO_0527413c_b286_4e9c_b2d0_03fb2a038dee"/>
                    <rdf:Description rdf:about="http://emmo.info/perspectives/emmo-semiotics.owl#EMMO_6f5af708_f825_4feb_a0d1_a8d813d3022b"/>
                    <rdf:Description rdf:about="http://emmo.info/perspectives/emmo-semiotics.owl#EMMO_b21a56ed_f969_4612_a6ec_cb7766f7f31d"/>
                </owl:unionOf>
            </owl:Class>
        </owl:equivalentClass>
        <rdfs:subClassOf>
            <owl:Restriction>
                <owl:onProperty>
                    <rdf:Description>
                        <owl:inverseOf rdf:resource="http://emmo.info/perspectives/emmo-processual.owl#EMMO_c5aae418_1622_4d02_93c5_21159e28e6c1"/>
                    </rdf:Description>
                </owl:onProperty>
                <owl:someValuesFrom rdf:resource="http://emmo.info/perspectives/emmo-semiotics.owl#EMMO_008fd3b2_4013_451f_8827_52bceab11841"/>
            </owl:Restriction>
        </rdfs:subClassOf>
        <emmo-annotations:EMMO_967080e5_2f42_4eb2_a3a9_c58143e835f9>The class of individuals that stands for semiotic objects, i.e. objects that take part on a semiotic process.</emmo-annotations:EMMO_967080e5_2f42_4eb2_a3a9_c58143e835f9>
        <rdfs:comment>Semiotic subclasse are defined using Peirce&apos;s semiotic theory.

&quot;Namely, a sign is something, A, which brings something, B, its interpretant sign determined or created by it, into the same sort of correspondence with something, C, its object, as that in which itself stands to C.&quot; (Peirce 1902, NEM 4, 20–21).

The triadic elements:
- &apos;sign&apos;: the sign A (e.g. a name)
- &apos;interpretant&apos;: the sign B as the effects of the sign A on the interpreter (e.g. the mental concept of what a name means)
- &apos;object&apos;: the object C (e.g. the entity to which the sign A and B refer to)

This class includes also the &apos;interpeter&apos; i.e. the entity that connects the &apos;sign&apos; to the &apos;object&apos;</rdfs:comment>
        <rdfs:label xml:lang="en">Semiotic</rdfs:label>
    </owl:Class>
    


    <!-- http://emmo.info/perspectives/emmo-semiotics.owl#EMMO_d7788d1a_020d_4c78_85a1_13563fcec168 -->

    <owl:Class rdf:about="http://emmo.info/perspectives/emmo-semiotics.owl#EMMO_d7788d1a_020d_4c78_85a1_13563fcec168">
        <emmo-annotations:EMMO_967080e5_2f42_4eb2_a3a9_c58143e835f9>A &apos;sign&apos; that stands for an &apos;object&apos; by resembling or imitating it, in shape or by sharing a similar logical structure.</emmo-annotations:EMMO_967080e5_2f42_4eb2_a3a9_c58143e835f9>
        <emmo-annotations:EMMO_b432d2d5_25f4_4165_99c5_5935a7763c1a>A picture that reproduces the aspect of a person. 

An equation that reproduces the logical connection of the properties of a physical entity.</emmo-annotations:EMMO_b432d2d5_25f4_4165_99c5_5935a7763c1a>
        <rdfs:label xml:lang="en">Icon</rdfs:label>
    </owl:Class>
</rdf:RDF>



<!-- Generated by the OWL API (version 4.5.9.2019-02-01T07:24:44Z) https://github.com/owlcs/owlapi -->

