@prefix : <http://emmo.info/emmo#> .
@prefix owl: <http://www.w3.org/2002/07/owl#> .
@prefix rdf: <http://www.w3.org/1999/02/22-rdf-syntax-ns#> .
@prefix xml: <http://www.w3.org/XML/1998/namespace> .
@prefix xsd: <http://www.w3.org/2001/XMLSchema#> .
@prefix rdfs: <http://www.w3.org/2000/01/rdf-schema#> .
@prefix skos: <http://www.w3.org/2004/02/skos/core#> .
@prefix dcterms: <http://purl.org/dc/terms/> .
@base <http://emmo.info/emmo/middle/holistic> .

<http://emmo.info/emmo/middle/holistic> rdf:type owl:Ontology ;
                                         owl:versionIRI <http://emmo.info/emmo/1.0.0-beta/middle/holistic> ;
                                         owl:imports <http://emmo.info/emmo/1.0.0-beta/middle/perspective> ;
                                         dcterms:abstract """Defines the holistic perspective which include process and the role of its participants.

Processes are 4D object's that unfolds in time in a way that has a meaning to the ontologist with participants who's role is assigned by the ontologist."""@en ;
                                         dcterms:contributor "Adham Hashibon, Fraunhofer IWM, DE" ,
                                                             "Georg Schmitz, Access, DE" ,
                                                             "Gerhard Goldbeck, Goldbeck Consulting Ltd (UK)" ,
                                                             "Jesper Friis, SINTEF, NO" ;
                                         dcterms:creator "Emanuele Ghedini, University of Bologna, IT" ;
                                         dcterms:license "https://creativecommons.org/licenses/by/4.0/legalcode" ;
                                         dcterms:publisher "EMMC ASBL" ;
                                         dcterms:title "Holistic"@en ;
                                         rdfs:comment """Contacts:
Gerhard Goldbeck
Goldbeck Consulting Ltd (UK)
email: gerhard@goldbeck-consulting.com

Emanuele Ghedini
University of Bologna (IT)
email: emanuele.ghedini@unibo.it"""@en ,
                                                      "The EMMO requires FacT++ reasoner plugin in order to visualize all inferences and class hierarchy (ctrl+R hotkey in Protege)."@en ;
                                         owl:versionInfo "1.0.0-beta" .

#################################################################
#    Object Properties
#################################################################

###  http://emmo.info/emmo#EMMO_3d88eccc_c9fc_498e_b6e2_c8a0984c9505
:EMMO_3d88eccc_c9fc_498e_b6e2_c8a0984c9505 rdf:type owl:ObjectProperty ;
                                           rdfs:subPropertyOf :EMMO_ae2d1a96_bfa1_409a_a7d2_03d69e8a125a ;
                                           :EMMO_967080e5_2f42_4eb2_a3a9_c58143e835f9 "A participant that overlaps only partially with the process." ;
                                           skos:prefLabel "hasPartialParticipant"@en .


###  http://emmo.info/emmo#EMMO_ae2d1a96_bfa1_409a_a7d2_03d69e8a125a
:EMMO_ae2d1a96_bfa1_409a_a7d2_03d69e8a125a rdf:type owl:ObjectProperty ;
                                           rdfs:subPropertyOf :EMMO_d893d373_b579_4867_841e_1c2b31a8d2c6 ;
                                           rdfs:domain :EMMO_43e9a05d_98af_41b4_92f6_00f79a09bfce ;
                                           rdfs:range :EMMO_49804605_c0fe_4538_abda_f70ba1dc8a5d ;
                                           :EMMO_967080e5_2f42_4eb2_a3a9_c58143e835f9 "The relation between a process and an object participating to it, i.e. that is relevant to the process itself."@en ;
                                           rdfs:comment """Participation is a parthood relation: you must be intersect the process to contribute to it.

Participation is not under direct parthood since a process is not strictly related to reductionism, but it's a way to categorize temporal regions by the interpreters."""@en ;
                                           skos:prefLabel "hasParticipant"@en .


###  http://emmo.info/emmo#EMMO_af9752c8_b6ec_4c03_b6a4_a581f306e089
:EMMO_af9752c8_b6ec_4c03_b6a4_a581f306e089 rdf:type owl:ObjectProperty ;
                                           rdfs:subPropertyOf :EMMO_17e27c22_37e1_468c_9dd7_95e137f73e7f ,
                                                              :EMMO_ae2d1a96_bfa1_409a_a7d2_03d69e8a125a ;
                                           :EMMO_967080e5_2f42_4eb2_a3a9_c58143e835f9 "A participant whose 4D extension is totally contained within the process." ;
                                           skos:prefLabel "hasFullParticipant"@en .


###  http://emmo.info/emmo#EMMO_c5aae418_1622_4d02_93c5_21159e28e6c1
:EMMO_c5aae418_1622_4d02_93c5_21159e28e6c1 rdf:type owl:ObjectProperty ;
                                           rdfs:subPropertyOf :EMMO_9380ab64_0363_4804_b13f_3a8a94119a76 ,
                                                              :EMMO_af9752c8_b6ec_4c03_b6a4_a581f306e089 ;
                                           skos:prefLabel "hasProperParticipant"@en .


#################################################################
#    Classes
#################################################################

###  http://emmo.info/emmo#EMMO_0277f24a_ea7f_4917_81b7_fb0406c8fc62
:EMMO_0277f24a_ea7f_4917_81b7_fb0406c8fc62 rdf:type owl:Class ;
                                           owl:equivalentClass [ rdf:type owl:Class ;
                                                                 owl:unionOf ( :EMMO_43e9a05d_98af_41b4_92f6_00f79a09bfce
                                                                               :EMMO_49804605_c0fe_4538_abda_f70ba1dc8a5d
                                                                             )
                                                               ] ;
                                           rdfs:subClassOf :EMMO_49267eba_5548_4163_8f36_518d65b583f9 ;
                                           :EMMO_967080e5_2f42_4eb2_a3a9_c58143e835f9 "A union of classes that categorize physicals under a holistic perspective: the interest is on the whole 4D object (process) and the role of its 4D parts (participants) without going further into specifying the spatial hierarchy or the temporal position of each part."@en ;
                                           rdfs:comment """An holistic perspective considers each part of the whole as equally important, without the need of a granularity hierarchy (in time or space).

A molecule of a body can have role in the body evolution, without caring if its part of a specific organ and without specifying the time interval in which this role occurred.

This class allows the picking of parts without necessarily going trough a rigid hierarchy of spatial compositions (e.g. body -> organ -> cell -> molecule) or temporal composition."""@en ;
                                           skos:prefLabel "Holistic"@en .

[ rdf:type owl:Axiom ;
   owl:annotatedSource :EMMO_0277f24a_ea7f_4917_81b7_fb0406c8fc62 ;
   owl:annotatedProperty skos:prefLabel ;
   owl:annotatedTarget "Holistic"@en ;
   :EMMO_705f27ae_954c_4f13_98aa_18473fc52b25 "Holism (from Greek ὅλος holos \"all, whole, entire\")."@en
 ] .


###  http://emmo.info/emmo#EMMO_43e9a05d_98af_41b4_92f6_00f79a09bfce
:EMMO_43e9a05d_98af_41b4_92f6_00f79a09bfce rdf:type owl:Class ;
                                           rdfs:subClassOf :EMMO_c5ddfdba_c074_4aa4_ad6b_1ac4942d300d ,
                                                           [ rdf:type owl:Restriction ;
                                                             owl:onProperty :EMMO_ae2d1a96_bfa1_409a_a7d2_03d69e8a125a ;
                                                             owl:someValuesFrom :EMMO_49804605_c0fe_4538_abda_f70ba1dc8a5d
                                                           ] ;
                                           :EMMO_967080e5_2f42_4eb2_a3a9_c58143e835f9 "A temporal part of a physical that identifies a particular type of evolution in time."@en ;
                                           rdfs:comment """Following the common definition of process, the reader may think that every 'Physical' should be a process, since every 4D object always has a time dimension. 

However, in the EMMO we restrict the meaning of the word process to 'Physical'-s whose evolution in time have a particular meaning for the ontologist (i.e. every 4D object unfolds in time, but not every 4D object may be of interest for the ontologist). 

A 'Process' is not only something that unfolds in time (which is automatically represented in a 4D ontology), but something that has a meaning for the ontologist (i.e. that the ontologist can separate from the rest of the 4D physical for any reason)."""@en ;
                                           skos:prefLabel "Process"@en .


###  http://emmo.info/emmo#EMMO_49804605_c0fe_4538_abda_f70ba1dc8a5d
:EMMO_49804605_c0fe_4538_abda_f70ba1dc8a5d rdf:type owl:Class ;
                                           rdfs:subClassOf :EMMO_c5ddfdba_c074_4aa4_ad6b_1ac4942d300d ,
                                                           [ rdf:type owl:Restriction ;
                                                             owl:onProperty [ owl:inverseOf :EMMO_ae2d1a96_bfa1_409a_a7d2_03d69e8a125a
                                                                            ] ;
                                                             owl:someValuesFrom :EMMO_43e9a05d_98af_41b4_92f6_00f79a09bfce
                                                           ] ;
                                           :EMMO_967080e5_2f42_4eb2_a3a9_c58143e835f9 "A portion of a 'Process' that participates to the process with a specific role."@en ;
                                           rdfs:comment """In the EMMO the relation of participation to a process falls under mereotopology.

Since topological connection means causality, then the only way for a real world object to participate to a process is to be a part of it."""@en ;
                                           skos:prefLabel "Participant"@en .


###  http://emmo.info/emmo/middle/manufacturing#65a007dc_2550_46b0_b394_3346c67fbb69
<http://emmo.info/emmo/middle/manufacturing#65a007dc_2550_46b0_b394_3346c67fbb69> rdf:type owl:Class ;
                                                                                  rdfs:subClassOf :EMMO_43e9a05d_98af_41b4_92f6_00f79a09bfce ;
                                                                                  :EMMO_967080e5_2f42_4eb2_a3a9_c58143e835f9 "An object that is made of a set of sub objects working together as parts of a mechanism or an interconnecting network; a complex whole."@en ;
                                                                                  rdfs:comment "A system is considered a process since it is conceived as an aggregate of things that 'work' (or interact) together, end then extending in time through distinct temporal parts."@en ;
                                                                                  skos:prefLabel "System"@en .

[ rdf:type owl:Axiom ;
   owl:annotatedSource <http://emmo.info/emmo/middle/manufacturing#65a007dc_2550_46b0_b394_3346c67fbb69> ;
   owl:annotatedProperty skos:prefLabel ;
   owl:annotatedTarget "System"@en ;
   :EMMO_705f27ae_954c_4f13_98aa_18473fc52b25 "From Latin systema, from Greek sustēma, from sun- ‘with’ + histanai ‘set up’."@en
 ] .


###  Generated by the OWL API (version 4.5.9.2019-02-01T07:24:44Z) https://github.com/owlcs/owlapi
