<?xml version="1.0"?>
<rdf:RDF xmlns="http://emmo.info/emmo/middle/models#"
     xml:base="http://emmo.info/emmo/middle/models"
     xmlns:rdf="http://www.w3.org/1999/02/22-rdf-syntax-ns#"
     xmlns:owl="http://www.w3.org/2002/07/owl#"
     xmlns:xml="http://www.w3.org/XML/1998/namespace"
     xmlns:xsd="http://www.w3.org/2001/XMLSchema#"
     xmlns:annotations="http://emmo.info/emmo/top/annotations#"
     xmlns:rdfs="http://www.w3.org/2000/01/rdf-schema#"
     xmlns:units="http://emmo.info/emmo/middle/metrology#">
    <owl:Ontology rdf:about="http://emmo.info/emmo/middle/models">
        <owl:versionIRI rdf:resource="http://emmo.info/emmo/marketplace-1.0.1/middle/models"/>
        <owl:imports rdf:resource="http://emmo.info/emmo/marketplace-1.0.1/middle/metrology"/>
        <annotations:EMMO_cd5fb112_7ee7_4120_a35d_3ca3e6c3f4ab>Emanuele Ghedini (University of Bologna, IT)
Gerhard Goldbeck (GCL Ltd, UK)
Adham Hashibon (Fraunhofer IWM, DE)
Georg Schmitz (Access, DE)
Jesper Friis (SINTEF, NO)</annotations:EMMO_cd5fb112_7ee7_4120_a35d_3ca3e6c3f4ab>
        <annotations:EMMO_5525a055_dda5_4556_8b91_f0d22fa676cc>EMMO is released under a Creative Commons license Attribution 4.0 International (CC BY 4.0)

https://creativecommons.org/licenses/by/4.0/legalcode</annotations:EMMO_5525a055_dda5_4556_8b91_f0d22fa676cc>
        <owl:versionInfo>The European Materials Modelling Ontology

Version 1.0.0-alpha2</owl:versionInfo>
        <rdfs:comment xml:lang="en">Contacts:
Gerhard Goldbeck
Goldbeck Consulting Ltd (UK)
email: gerhard@goldbeck-consulting.com

Emanuele Ghedini
University of Bologna (IT)
email: emanuele.ghedini@unibo.it</rdfs:comment>
        <rdfs:comment>The EMMO requires FacT++ reasoner plugin in order to visualize all inferences and class hierarchy (ctrl+R hotkey in Protege).</rdfs:comment>
        <rdfs:comment>European Materials and Modelling Ontology (EMMO)

EMMO is a multidisciplinary effort to develop a standard representational framework (the ontology) based on current materials modelling knowledge, including physical sciences, analytical philosophy and information and communication technologies. 

It provides the connection between the physical world, materials characterisation world and materials modelling world.</rdfs:comment>
    </owl:Ontology>
    


    <!-- 
    ///////////////////////////////////////////////////////////////////////////////////////
    //
    // Object Properties
    //
    ///////////////////////////////////////////////////////////////////////////////////////
     -->

    


    <!-- http://emmo.info/emmo/middle/models#EMMO_24c71baf_6db6_48b9_86c8_8c70cf36db0c -->

    <owl:ObjectProperty rdf:about="http://emmo.info/emmo/middle/models#EMMO_24c71baf_6db6_48b9_86c8_8c70cf36db0c">
        <rdfs:subPropertyOf rdf:resource="http://emmo.info/emmo/middle/semiotics#EMMO_39c3815d_8cae_4c8f_b2ff_eeba24bec455"/>
        <rdfs:label xml:lang="en">hasModel</rdfs:label>
    </owl:ObjectProperty>
    


    <!-- 
    ///////////////////////////////////////////////////////////////////////////////////////
    //
    // Classes
    //
    ///////////////////////////////////////////////////////////////////////////////////////
     -->

    


    <!-- http://emmo.info/emmo/middle/models#EMMO_22522299_4091_4d1f_82a2_3890492df6db -->

    <owl:Class rdf:about="http://emmo.info/emmo/middle/models#EMMO_22522299_4091_4d1f_82a2_3890492df6db">
        <rdfs:subClassOf rdf:resource="http://emmo.info/emmo/middle/properties#EMMO_10a5fd39_06aa_4648_9e70_f962a9cb2069"/>
        <rdfs:subClassOf>
            <owl:Restriction>
                <owl:onProperty rdf:resource="http://emmo.info/emmo/middle/holistic#EMMO_ae2d1a96_bfa1_409a_a7d2_03d69e8a125a"/>
                <owl:someValuesFrom rdf:resource="http://emmo.info/emmo/middle/models#EMMO_314d0bd5_67ed_437e_a609_36d46147cea7"/>
            </owl:Restriction>
        </rdfs:subClassOf>
        <annotations:EMMO_967080e5_2f42_4eb2_a3a9_c58143e835f9>An experiment is a process that is intended to replicate a physical phenomenon in a controlled environment.</annotations:EMMO_967080e5_2f42_4eb2_a3a9_c58143e835f9>
        <rdfs:label xml:lang="en">Experiment</rdfs:label>
    </owl:Class>
    


    <!-- http://emmo.info/emmo/middle/models#EMMO_27c5d8c6_8af7_4d63_beb1_ec37cd8b3fa3 -->

    <owl:Class rdf:about="http://emmo.info/emmo/middle/models#EMMO_27c5d8c6_8af7_4d63_beb1_ec37cd8b3fa3">
        <rdfs:subClassOf rdf:resource="http://emmo.info/emmo/middle/math#EMMO_e56ee3eb_7609_4ae1_8bed_51974f0960a6"/>
        <rdfs:subClassOf>
            <owl:Restriction>
                <owl:onProperty rdf:resource="http://emmo.info/emmo/middle/reductionistic#EMMO_b2282816_b7a3_44c6_b2cb_3feff1ceb7fe"/>
                <owl:someValuesFrom rdf:resource="http://emmo.info/emmo/middle/metrology#EMMO_02c0621e_a527_4790_8a0f_2bb51973c819"/>
            </owl:Restriction>
        </rdfs:subClassOf>
        <rdfs:subClassOf>
            <owl:Restriction>
                <owl:onProperty>
                    <rdf:Description>
                        <owl:inverseOf rdf:resource="http://emmo.info/emmo/middle/models#EMMO_24c71baf_6db6_48b9_86c8_8c70cf36db0c"/>
                    </rdf:Description>
                </owl:onProperty>
                <owl:someValuesFrom rdf:resource="http://emmo.info/emmo/middle/models#EMMO_314d0bd5_67ed_437e_a609_36d46147cea7"/>
            </owl:Restriction>
        </rdfs:subClassOf>
        <annotations:EMMO_967080e5_2f42_4eb2_a3a9_c58143e835f9>An &apos;equation&apos; that stands for a &apos;physical_law&apos; by mathematically defining the relations between physics_quantities.</annotations:EMMO_967080e5_2f42_4eb2_a3a9_c58143e835f9>
        <rdfs:comment>The Newton&apos;s equation of motion.

The Schrodinger equation.

The Navier-Stokes equation.</rdfs:comment>
        <rdfs:label xml:lang="en">PhysicsEquation</rdfs:label>
    </owl:Class>
    


    <!-- http://emmo.info/emmo/middle/models#EMMO_314d0bd5_67ed_437e_a609_36d46147cea7 -->

    <owl:Class rdf:about="http://emmo.info/emmo/middle/models#EMMO_314d0bd5_67ed_437e_a609_36d46147cea7">
        <rdfs:subClassOf rdf:resource="http://emmo.info/emmo/middle/holistic#EMMO_43e9a05d_98af_41b4_92f6_00f79a09bfce"/>
        <annotations:EMMO_967080e5_2f42_4eb2_a3a9_c58143e835f9>A &apos;process&apos; that is recognized by physical sciences and is catogrized accordingly.</annotations:EMMO_967080e5_2f42_4eb2_a3a9_c58143e835f9>
        <rdfs:comment>While every &apos;process&apos; in the EMMO involves physical objects, this class is devoted to represent real world objects that express a phenomena relevant for the ontologist.</rdfs:comment>
        <rdfs:label xml:lang="en">PhysicalPhenomenon</rdfs:label>
    </owl:Class>
    


    <!-- http://emmo.info/emmo/middle/models#EMMO_4456a5d2_16a6_4ee1_9a8e_5c75956b28ea -->

    <owl:Class rdf:about="http://emmo.info/emmo/middle/models#EMMO_4456a5d2_16a6_4ee1_9a8e_5c75956b28ea">
        <rdfs:subClassOf rdf:resource="http://emmo.info/emmo/middle/models#EMMO_b29fd350_39aa_4af7_9459_3faa0544cba6"/>
        <annotations:EMMO_967080e5_2f42_4eb2_a3a9_c58143e835f9>A physics-based model based on a physics equation describing the behaviour of continuum volume.</annotations:EMMO_967080e5_2f42_4eb2_a3a9_c58143e835f9>
        <rdfs:label xml:lang="en">ContinuumModel</rdfs:label>
    </owl:Class>
    


    <!-- http://emmo.info/emmo/middle/models#EMMO_53935db0_af45_4426_b9e9_244a0d77db00 -->

    <owl:Class rdf:about="http://emmo.info/emmo/middle/models#EMMO_53935db0_af45_4426_b9e9_244a0d77db00">
        <rdfs:subClassOf rdf:resource="http://emmo.info/emmo/middle/models#EMMO_b29fd350_39aa_4af7_9459_3faa0544cba6"/>
        <annotations:EMMO_967080e5_2f42_4eb2_a3a9_c58143e835f9>A physics-based model based on a physics equation describing the behaviour of mesoscopic entities, i.e. a set of bounded atoms like a molecule, bead or nanoparticle.</annotations:EMMO_967080e5_2f42_4eb2_a3a9_c58143e835f9>
        <rdfs:label xml:lang="en">MesoscopicModel</rdfs:label>
    </owl:Class>
    


    <!-- http://emmo.info/emmo/middle/models#EMMO_6c739b1a_a774_4416_bb31_1961486fa9ed -->

    <owl:Class rdf:about="http://emmo.info/emmo/middle/models#EMMO_6c739b1a_a774_4416_bb31_1961486fa9ed">
        <rdfs:subClassOf rdf:resource="http://emmo.info/emmo/middle/properties#EMMO_10a5fd39_06aa_4648_9e70_f962a9cb2069"/>
        <annotations:EMMO_967080e5_2f42_4eb2_a3a9_c58143e835f9>The &apos;semiosis&apos; process of interpreting a &apos;physical&apos; and provide a complec sign, &apos;theory&apos; that stands for it and explain it to another interpreter.</annotations:EMMO_967080e5_2f42_4eb2_a3a9_c58143e835f9>
        <rdfs:label xml:lang="en">Theorization</rdfs:label>
    </owl:Class>
    


    <!-- http://emmo.info/emmo/middle/models#EMMO_6eca09be_17e9_445e_abc9_000aa61b7a11 -->

    <owl:Class rdf:about="http://emmo.info/emmo/middle/models#EMMO_6eca09be_17e9_445e_abc9_000aa61b7a11">
        <rdfs:subClassOf rdf:resource="http://emmo.info/emmo/middle/models#EMMO_b29fd350_39aa_4af7_9459_3faa0544cba6"/>
        <annotations:EMMO_967080e5_2f42_4eb2_a3a9_c58143e835f9>A physics-based model based on a physics equation describing the behaviour of electrons.</annotations:EMMO_967080e5_2f42_4eb2_a3a9_c58143e835f9>
        <annotations:EMMO_b432d2d5_25f4_4165_99c5_5935a7763c1a>Density functional theory.
Hartree-Fock.</annotations:EMMO_b432d2d5_25f4_4165_99c5_5935a7763c1a>
        <rdfs:label xml:lang="en">ElectronicModel</rdfs:label>
    </owl:Class>
    


    <!-- http://emmo.info/emmo/middle/models#EMMO_84cadc45_6758_46f2_ba2a_5ead65c70213 -->

    <owl:Class rdf:about="http://emmo.info/emmo/middle/models#EMMO_84cadc45_6758_46f2_ba2a_5ead65c70213">
        <rdfs:subClassOf rdf:resource="http://emmo.info/emmo/middle/models#EMMO_b29fd350_39aa_4af7_9459_3faa0544cba6"/>
        <annotations:EMMO_967080e5_2f42_4eb2_a3a9_c58143e835f9>A physics-based model based on a physics equation describing the behaviour of atoms.</annotations:EMMO_967080e5_2f42_4eb2_a3a9_c58143e835f9>
        <rdfs:label xml:lang="en">AtomisticModel</rdfs:label>
    </owl:Class>
    


    <!-- http://emmo.info/emmo/middle/models#EMMO_8d2d9374_ef3a_47e6_8595_6bc208e07519 -->

    <owl:Class rdf:about="http://emmo.info/emmo/middle/models#EMMO_8d2d9374_ef3a_47e6_8595_6bc208e07519">
        <rdfs:subClassOf rdf:resource="http://emmo.info/emmo/middle/semiotics#EMMO_35d2e130_6e01_41ed_94f7_00b333d46cf9"/>
        <annotations:EMMO_967080e5_2f42_4eb2_a3a9_c58143e835f9>A &apos;conventional&apos; that stand for a &apos;physical&apos;.</annotations:EMMO_967080e5_2f42_4eb2_a3a9_c58143e835f9>
        <rdfs:comment>The &apos;theory&apos; is e.g. a proposition, a book or a paper whose sub-symbols suggest in the mind of the interpreter an interpretant structure that can represent a &apos;physical&apos;.

It is not an &apos;icon&apos; (like a math equation), because it has no common resemblance or logical structure with the &apos;physical&apos;.

In Peirce semiotics: legisign-symbol-argument</rdfs:comment>
        <rdfs:label xml:lang="en">Theory</rdfs:label>
    </owl:Class>
    


    <!-- http://emmo.info/emmo/middle/models#EMMO_939483b1_0148_43d1_8b35_851d2cd5d939 -->

    <owl:Class rdf:about="http://emmo.info/emmo/middle/models#EMMO_939483b1_0148_43d1_8b35_851d2cd5d939">
        <owl:equivalentClass>
            <owl:Restriction>
                <owl:onProperty>
                    <rdf:Description>
                        <owl:inverseOf rdf:resource="http://emmo.info/emmo/middle/models#EMMO_24c71baf_6db6_48b9_86c8_8c70cf36db0c"/>
                    </rdf:Description>
                </owl:onProperty>
                <owl:someValuesFrom rdf:resource="http://emmo.info/emmo/top/physical#EMMO_c5ddfdba_c074_4aa4_ad6b_1ac4942d300d"/>
            </owl:Restriction>
        </owl:equivalentClass>
        <annotations:EMMO_967080e5_2f42_4eb2_a3a9_c58143e835f9>A &apos;sign&apos; that not only stands for a &apos;physical&apos; or a &apos;process&apos;, but it is also a simplified representation, aimed to assist calculations for its description or for predictions of its behaviour.

A &apos;model&apos; represents a &apos;physical&apos; or a &apos;process&apos; by direct similitude (e.g. small scale replica) or by capturing in a logical framework the relations between its properties (e.g. mathematical model).</annotations:EMMO_967080e5_2f42_4eb2_a3a9_c58143e835f9>
        <rdfs:comment>A &apos;model&apos; prediction is always a prediction of the properties of an entity, since an entity is known by an interpreter only through perception.</rdfs:comment>
        <rdfs:label xml:lang="en">Model</rdfs:label>
    </owl:Class>
    


    <!-- http://emmo.info/emmo/middle/models#EMMO_9c32fd69_f480_4130_83b3_fb25d9face14 -->

    <owl:Class rdf:about="http://emmo.info/emmo/middle/models#EMMO_9c32fd69_f480_4130_83b3_fb25d9face14">
        <rdfs:subClassOf rdf:resource="http://emmo.info/emmo/middle/models#EMMO_db9a009e_f097_43f5_9520_6cbc07e7610b"/>
        <rdfs:label xml:lang="en">PhysicalLaw</rdfs:label>
    </owl:Class>
    


    <!-- http://emmo.info/emmo/middle/models#EMMO_a4b14b83_9392_4a5f_a2e8_b2b58793f59b -->

    <owl:Class rdf:about="http://emmo.info/emmo/middle/models#EMMO_a4b14b83_9392_4a5f_a2e8_b2b58793f59b">
        <rdfs:subClassOf rdf:resource="http://emmo.info/emmo/middle/models#EMMO_f7ed665b_c2e1_42bc_889b_6b42ed3a36f0"/>
        <annotations:EMMO_967080e5_2f42_4eb2_a3a9_c58143e835f9>A computational model that uses data to create new insight into the behaviour of a system.</annotations:EMMO_967080e5_2f42_4eb2_a3a9_c58143e835f9>
        <rdfs:label xml:lang="en">DataBasedModel</rdfs:label>
    </owl:Class>
    


    <!-- http://emmo.info/emmo/middle/models#EMMO_b29fd350_39aa_4af7_9459_3faa0544cba6 -->

    <owl:Class rdf:about="http://emmo.info/emmo/middle/models#EMMO_b29fd350_39aa_4af7_9459_3faa0544cba6">
        <rdfs:subClassOf rdf:resource="http://emmo.info/emmo/middle/models#EMMO_f7ed665b_c2e1_42bc_889b_6b42ed3a36f0"/>
        <rdfs:subClassOf>
            <owl:Restriction>
                <owl:onProperty rdf:resource="http://emmo.info/emmo/top/physical#EMMO_f68030be_94b8_4c61_a161_886468558054"/>
                <owl:someValuesFrom rdf:resource="http://emmo.info/emmo/middle/models#EMMO_27c5d8c6_8af7_4d63_beb1_ec37cd8b3fa3"/>
            </owl:Restriction>
        </rdfs:subClassOf>
        <rdfs:subClassOf>
            <owl:Restriction>
                <owl:onProperty rdf:resource="http://emmo.info/emmo/top/physical#EMMO_f68030be_94b8_4c61_a161_886468558054"/>
                <owl:someValuesFrom rdf:resource="http://emmo.info/emmo/middle/models#EMMO_e5438930_04e7_4d42_ade5_3700d4a52ab7"/>
            </owl:Restriction>
        </rdfs:subClassOf>
        <annotations:EMMO_967080e5_2f42_4eb2_a3a9_c58143e835f9>A solvable set of one Physics Equation and one or more Materials Relations.</annotations:EMMO_967080e5_2f42_4eb2_a3a9_c58143e835f9>
        <rdfs:label xml:lang="en">PhysicsBasedModel</rdfs:label>
    </owl:Class>
    


    <!-- http://emmo.info/emmo/middle/models#EMMO_db9a009e_f097_43f5_9520_6cbc07e7610b -->

    <owl:Class rdf:about="http://emmo.info/emmo/middle/models#EMMO_db9a009e_f097_43f5_9520_6cbc07e7610b">
        <rdfs:subClassOf rdf:resource="http://emmo.info/emmo/middle/models#EMMO_8d2d9374_ef3a_47e6_8595_6bc208e07519"/>
        <rdfs:label xml:lang="en">NaturalLaw</rdfs:label>
    </owl:Class>
    


    <!-- http://emmo.info/emmo/middle/models#EMMO_e5438930_04e7_4d42_ade5_3700d4a52ab7 -->

    <owl:Class rdf:about="http://emmo.info/emmo/middle/models#EMMO_e5438930_04e7_4d42_ade5_3700d4a52ab7">
        <rdfs:subClassOf rdf:resource="http://emmo.info/emmo/middle/math#EMMO_e56ee3eb_7609_4ae1_8bed_51974f0960a6"/>
        <rdfs:subClassOf>
            <owl:Restriction>
                <owl:onProperty rdf:resource="http://emmo.info/emmo/middle/reductionistic#EMMO_b2282816_b7a3_44c6_b2cb_3feff1ceb7fe"/>
                <owl:someValuesFrom rdf:resource="http://emmo.info/emmo/middle/metrology#EMMO_02c0621e_a527_4790_8a0f_2bb51973c819"/>
            </owl:Restriction>
        </rdfs:subClassOf>
        <annotations:EMMO_967080e5_2f42_4eb2_a3a9_c58143e835f9>An &apos;equation&apos; that stands for a physical assumption specific to a material, and provides an expression for a &apos;physics_quantity&apos; (the dependent variable) as function of other variables, physics_quantity or data (independent variables).</annotations:EMMO_967080e5_2f42_4eb2_a3a9_c58143e835f9>
        <annotations:EMMO_b432d2d5_25f4_4165_99c5_5935a7763c1a>The Lennard-Jones potential.

A force field.

An Hamiltonian.</annotations:EMMO_b432d2d5_25f4_4165_99c5_5935a7763c1a>
        <rdfs:comment>A material_relation can e.g. return a predefined number, return a database query, be an equation that depends on other physics_quantities.</rdfs:comment>
        <rdfs:label xml:lang="en">MaterialRelation</rdfs:label>
    </owl:Class>
    


    <!-- http://emmo.info/emmo/middle/models#EMMO_f19ff3b4_6bfe_4c41_a2b2_9affd39c140b -->

    <owl:Class rdf:about="http://emmo.info/emmo/middle/models#EMMO_f19ff3b4_6bfe_4c41_a2b2_9affd39c140b">
        <rdfs:subClassOf rdf:resource="http://emmo.info/emmo/middle/models#EMMO_db9a009e_f097_43f5_9520_6cbc07e7610b"/>
        <rdfs:label xml:lang="en">MaterialLaw</rdfs:label>
    </owl:Class>
    


    <!-- http://emmo.info/emmo/middle/models#EMMO_f7ed665b_c2e1_42bc_889b_6b42ed3a36f0 -->

    <owl:Class rdf:about="http://emmo.info/emmo/middle/models#EMMO_f7ed665b_c2e1_42bc_889b_6b42ed3a36f0">
        <owl:equivalentClass>
            <owl:Class>
                <owl:intersectionOf rdf:parseType="Collection">
                    <rdf:Description rdf:about="http://emmo.info/emmo/middle/math#EMMO_54ee6b5e_5261_44a8_86eb_5717e7fdb9d0"/>
                    <rdf:Description rdf:about="http://emmo.info/emmo/middle/models#EMMO_939483b1_0148_43d1_8b35_851d2cd5d939"/>
                </owl:intersectionOf>
            </owl:Class>
        </owl:equivalentClass>
        <rdfs:comment>A mathematical model can be defined as a description of a system using mathematical concepts and language to facilitate proper explanation of a system or to study the effects of different components and to make predictions on patterns of behaviour. 

Abramowitz and Stegun, 1968</rdfs:comment>
        <rdfs:label xml:lang="en">MathematicalModel</rdfs:label>
    </owl:Class>
</rdf:RDF>



<!-- Generated by the OWL API (version 4.2.8.20170104-2310) https://github.com/owlcs/owlapi -->

