<?xml version="1.0"?>
<rdf:RDF xmlns="http://emmo.info/domains/emmo-physical-constants.owl#"
     xml:base="http://emmo.info/domains/emmo-physical-constants.owl"
     xmlns:rdf="http://www.w3.org/1999/02/22-rdf-syntax-ns#"
     xmlns:terms="http://purl.org/dc/terms/"
     xmlns:owl="http://www.w3.org/2002/07/owl#"
     xmlns:xml="http://www.w3.org/XML/1998/namespace"
     xmlns:xsd="http://www.w3.org/2001/XMLSchema#"
     xmlns:rdfs="http://www.w3.org/2000/01/rdf-schema#"
     xmlns:dc="http://purl.org/dc/elements/1.1/"
     xmlns:emmo-annotations="http://emmo.info/base/emmo-annotations.owl#">
    <owl:Ontology rdf:about="http://emmo.info/domains/emmo-physical-constants.owl">
        <owl:imports rdf:resource="http://emmo.info/domains/emmo-si-units.owl"/>
        <emmo-annotations:EMMO_5525a055_dda5_4556_8b91_f0d22fa676cc>EMMO is released under a Creative Commons license Attribution 4.0 International (CC BY 4.0)

https://creativecommons.org/licenses/by/4.0/legalcode</emmo-annotations:EMMO_5525a055_dda5_4556_8b91_f0d22fa676cc>
        <rdfs:comment>European Materials and Modelling Ontology (EMMO)

EMMO is a multidisciplinary effort to develop a standard representational framework (the ontology) based on current materials modelling knowledge, including physical sciences, analytical philosophy and information and communication technologies.

It provides the connection between the physical world, materials characterisation world and materials modelling world.</rdfs:comment>
        <emmo-annotations:EMMO_cd5fb112_7ee7_4120_a35d_3ca3e6c3f4ab>Emanuele Ghedini (University of Bologna, IT)
Gerhard Goldbeck (GCL Ltd, UK)
Adham Hashibon (Fraunhofer IWM, DE)
Georg Schmitz (Access, DE)
Jesper Friis (SINTEF, NO)</emmo-annotations:EMMO_cd5fb112_7ee7_4120_a35d_3ca3e6c3f4ab>
        <rdfs:comment>Contacts:
Gerhard Goldbeck
Goldbeck Consulting Ltd (UK)
email: gerhard@goldbeck-consulting.com

Emanuele Ghedini
University of Bologna (IT)
email: emanuele.ghedini@unibo.it</rdfs:comment>
        <rdfs:comment>The EMMO requires FacT++ reasoner plugin in order to visualize all inferences and class hierarchy (ctrl+R hotkey in Protege).</rdfs:comment>
    </owl:Ontology>
    


    <!-- 
    ///////////////////////////////////////////////////////////////////////////////////////
    //
    // Classes
    //
    ///////////////////////////////////////////////////////////////////////////////////////
     -->

    


    <!-- http://emmo.info/domains/emmo-physical-constants.owl#EMMO_176cae33_b83e_4cd2_a6bc_281f42f0ccc8 -->

    <owl:Class rdf:about="http://emmo.info/domains/emmo-physical-constants.owl#EMMO_176cae33_b83e_4cd2_a6bc_281f42f0ccc8">
        <rdfs:subClassOf rdf:resource="http://emmo.info/domains/emmo-physical-constants.owl#EMMO_89762966_8076_4f7c_b745_f718d653e8e2"/>
        <emmo-annotations:EMMO_1f1b164d_ec6a_4faa_8d5e_88bda62316cc>http://physics.nist.gov/cuu/CODATA-Value_AvogadroConstant</emmo-annotations:EMMO_1f1b164d_ec6a_4faa_8d5e_88bda62316cc>
        <emmo-annotations:EMMO_6dd685dd_1895_46e4_b227_be9f7d643c25>http://dbpedia.org/page/Avogadro_constant</emmo-annotations:EMMO_6dd685dd_1895_46e4_b227_be9f7d643c25>
        <emmo-annotations:EMMO_fe015383_afb3_44a6_ae86_043628697aa2>https://doi.org/10.1351/goldbook.A00543</emmo-annotations:EMMO_fe015383_afb3_44a6_ae86_043628697aa2>
        <rdfs:comment>The DBpedia definition (http://dbpedia.org/page/Avogadro_constant) is outdated as May 20, 2019. It is now an exact quantity.</rdfs:comment>
        <rdfs:comment>The number of constituent particles, usually atoms or molecules, that are contained in the amount of substance given by one mole.</rdfs:comment>
        <rdfs:label xml:lang="en">AvogadroConstant</rdfs:label>
    </owl:Class>
    


    <!-- http://emmo.info/domains/emmo-physical-constants.owl#EMMO_3f15d200_c97b_42c8_8ac0_d81d150361e2 -->

    <owl:Class rdf:about="http://emmo.info/domains/emmo-physical-constants.owl#EMMO_3f15d200_c97b_42c8_8ac0_d81d150361e2">
        <rdfs:subClassOf rdf:resource="http://emmo.info/domains/emmo-units.owl#EMMO_b953f2b1_c8d1_4dd9_b630_d3ef6580c2bb"/>
        <rdfs:comment>Physical constants whos value must be measured and is therefore associated with an uncertainty.</rdfs:comment>
        <rdfs:label xml:lang="en">MeasuredConstant</rdfs:label>
    </owl:Class>
    


    <!-- http://emmo.info/domains/emmo-physical-constants.owl#EMMO_44fc8c60_7a9c_49af_a046_e1878c88862c -->

    <owl:Class rdf:about="http://emmo.info/domains/emmo-physical-constants.owl#EMMO_44fc8c60_7a9c_49af_a046_e1878c88862c">
        <rdfs:subClassOf rdf:resource="http://emmo.info/domains/emmo-physical-constants.owl#EMMO_3f15d200_c97b_42c8_8ac0_d81d150361e2"/>
        <rdfs:subClassOf rdf:resource="http://emmo.info/domains/emmo-units.owl#EMMO_ed4af7ae_63a2_497e_bb88_2309619ea405"/>
        <emmo-annotations:EMMO_1f1b164d_ec6a_4faa_8d5e_88bda62316cc>http://physics.nist.gov/cuu/CODATA-Value_ElectronMass</emmo-annotations:EMMO_1f1b164d_ec6a_4faa_8d5e_88bda62316cc>
        <emmo-annotations:EMMO_6dd685dd_1895_46e4_b227_be9f7d643c25>http://dbpedia.org/page/Electron_rest_mass</emmo-annotations:EMMO_6dd685dd_1895_46e4_b227_be9f7d643c25>
        <emmo-annotations:EMMO_fe015383_afb3_44a6_ae86_043628697aa2>https://doi.org/10.1351/goldbook.E02008</emmo-annotations:EMMO_fe015383_afb3_44a6_ae86_043628697aa2>
        <rdfs:comment>The rest mass of an electron.</rdfs:comment>
        <rdfs:label xml:lang="en">ElectronMass</rdfs:label>
    </owl:Class>
    


    <!-- http://emmo.info/domains/emmo-physical-constants.owl#EMMO_5186f2b2_e981_425d_8d87_0cbb753c0882 -->

    <owl:Class rdf:about="http://emmo.info/domains/emmo-physical-constants.owl#EMMO_5186f2b2_e981_425d_8d87_0cbb753c0882">
        <rdfs:subClassOf rdf:resource="http://emmo.info/domains/emmo-physical-constants.owl#EMMO_89762966_8076_4f7c_b745_f718d653e8e2"/>
        <emmo-annotations:EMMO_1f1b164d_ec6a_4faa_8d5e_88bda62316cc>http://physics.nist.gov/cuu/CODATA-Value_MolarGasConstant</emmo-annotations:EMMO_1f1b164d_ec6a_4faa_8d5e_88bda62316cc>
        <emmo-annotations:EMMO_6dd685dd_1895_46e4_b227_be9f7d643c25>http://dbpedia.org/page/Gas_constant</emmo-annotations:EMMO_6dd685dd_1895_46e4_b227_be9f7d643c25>
        <emmo-annotations:EMMO_fe015383_afb3_44a6_ae86_043628697aa2>https://doi.org/10.1351/goldbook.G02579</emmo-annotations:EMMO_fe015383_afb3_44a6_ae86_043628697aa2>
        <rdfs:comment>Equivalent to the Boltzmann constant, but expressed in units of energy per temperature increment per mole (rather than energy per temperature increment per particle).</rdfs:comment>
        <rdfs:label xml:lang="en">MolarGasConstant</rdfs:label>
    </owl:Class>
    


    <!-- http://emmo.info/domains/emmo-physical-constants.owl#EMMO_58a650f0_a638_4743_8439_535a325e5c4c -->

    <owl:Class rdf:about="http://emmo.info/domains/emmo-physical-constants.owl#EMMO_58a650f0_a638_4743_8439_535a325e5c4c">
        <rdfs:subClassOf rdf:resource="http://emmo.info/domains/emmo-physical-constants.owl#EMMO_89762966_8076_4f7c_b745_f718d653e8e2"/>
        <rdfs:subClassOf rdf:resource="http://emmo.info/domains/emmo-si-units.owl#EMMO_1604f495_328a_4f28_9962_f4cc210739dd"/>
        <emmo-annotations:EMMO_1f1b164d_ec6a_4faa_8d5e_88bda62316cc>http://physics.nist.gov/cuu/CODATA-Value_ElementaryCharge</emmo-annotations:EMMO_1f1b164d_ec6a_4faa_8d5e_88bda62316cc>
        <emmo-annotations:EMMO_6dd685dd_1895_46e4_b227_be9f7d643c25>http://dbpedia.org/page/Elementary_charge</emmo-annotations:EMMO_6dd685dd_1895_46e4_b227_be9f7d643c25>
        <emmo-annotations:EMMO_fe015383_afb3_44a6_ae86_043628697aa2>https://doi.org/10.1351/goldbook.E02032</emmo-annotations:EMMO_fe015383_afb3_44a6_ae86_043628697aa2>
        <rdfs:comment>The DBpedia definition (http://dbpedia.org/page/Elementary_charge) is outdated as May 20, 2019. It is now an exact quantity.</rdfs:comment>
        <rdfs:comment>The magnitude of the electric charge carried by a single electron.</rdfs:comment>
        <rdfs:label xml:lang="en">ElementaryCharge</rdfs:label>
    </owl:Class>
    


    <!-- http://emmo.info/domains/emmo-physical-constants.owl#EMMO_5c7261e7_4471_4422_9250_705770fdce79 -->

    <owl:Class rdf:about="http://emmo.info/domains/emmo-physical-constants.owl#EMMO_5c7261e7_4471_4422_9250_705770fdce79">
        <rdfs:subClassOf rdf:resource="http://emmo.info/domains/emmo-physical-constants.owl#EMMO_89762966_8076_4f7c_b745_f718d653e8e2"/>
        <emmo-annotations:EMMO_1f1b164d_ec6a_4faa_8d5e_88bda62316cc>http://physics.nist.gov/cuu/CODATA-Value_VonKlitzingConstant</emmo-annotations:EMMO_1f1b164d_ec6a_4faa_8d5e_88bda62316cc>
        <emmo-annotations:EMMO_70fe84ff_99b6_4206_a9fc_9a8931836d84>The von Klitzing constant is defined as Planck constant divided by the square of the elementary charge.</emmo-annotations:EMMO_70fe84ff_99b6_4206_a9fc_9a8931836d84>
        <rdfs:comment>Resistance quantum.</rdfs:comment>
        <rdfs:label xml:lang="en">VonKlitzingConstant</rdfs:label>
    </owl:Class>
    


    <!-- http://emmo.info/domains/emmo-physical-constants.owl#EMMO_61a32ae9_8200_473a_bd55_59a9899996f4 -->

    <owl:Class rdf:about="http://emmo.info/domains/emmo-physical-constants.owl#EMMO_61a32ae9_8200_473a_bd55_59a9899996f4">
        <rdfs:subClassOf rdf:resource="http://emmo.info/domains/emmo-si-units.owl#EMMO_0ee5779e_d798_4ee5_9bfe_c392d5bea112"/>
        <rdfs:subClassOf rdf:resource="http://emmo.info/domains/emmo-physical-constants.owl#EMMO_3f15d200_c97b_42c8_8ac0_d81d150361e2"/>
        <emmo-annotations:EMMO_1f1b164d_ec6a_4faa_8d5e_88bda62316cc>http://physics.nist.gov/cuu/CODATA-Value_ElectricConstant</emmo-annotations:EMMO_1f1b164d_ec6a_4faa_8d5e_88bda62316cc>
        <emmo-annotations:EMMO_fe015383_afb3_44a6_ae86_043628697aa2>https://doi.org/10.1351/goldbook.P04508</emmo-annotations:EMMO_fe015383_afb3_44a6_ae86_043628697aa2>
        <rdfs:comment>The DBpedia definition (http://dbpedia.org/page/Vacuum_permittivity) is outdated since May 20, 2019. It is now a measured constant.</rdfs:comment>
        <rdfs:comment>The value of the absolute dielectric permittivity of classical vacuum.</rdfs:comment>
        <rdfs:label xml:lang="en">VacuumElectricPermittivity</rdfs:label>
    </owl:Class>
    


    <!-- http://emmo.info/domains/emmo-physical-constants.owl#EMMO_76cc4efc_231e_42b4_be83_2547681caed6 -->

    <owl:Class rdf:about="http://emmo.info/domains/emmo-physical-constants.owl#EMMO_76cc4efc_231e_42b4_be83_2547681caed6">
        <rdfs:subClassOf rdf:resource="http://emmo.info/domains/emmo-si-units.owl#EMMO_66d01570_36dd_42fd_844d_29b81b029cd5"/>
        <rdfs:subClassOf rdf:resource="http://emmo.info/domains/emmo-physical-constants.owl#EMMO_89762966_8076_4f7c_b745_f718d653e8e2"/>
        <emmo-annotations:EMMO_1f1b164d_ec6a_4faa_8d5e_88bda62316cc>http://physics.nist.gov/cuu/CODATA-Value_PlankConstant</emmo-annotations:EMMO_1f1b164d_ec6a_4faa_8d5e_88bda62316cc>
        <emmo-annotations:EMMO_6dd685dd_1895_46e4_b227_be9f7d643c25>http://dbpedia.org/page/Planck_constant</emmo-annotations:EMMO_6dd685dd_1895_46e4_b227_be9f7d643c25>
        <emmo-annotations:EMMO_fe015383_afb3_44a6_ae86_043628697aa2>https://doi.org/10.1351/goldbook.P04685</emmo-annotations:EMMO_fe015383_afb3_44a6_ae86_043628697aa2>
        <rdfs:comment>The quantum of action.</rdfs:comment>
        <rdfs:label xml:lang="en">PlanckConstant</rdfs:label>
    </owl:Class>
    


    <!-- http://emmo.info/domains/emmo-physical-constants.owl#EMMO_89762966_8076_4f7c_b745_f718d653e8e2 -->

    <owl:Class rdf:about="http://emmo.info/domains/emmo-physical-constants.owl#EMMO_89762966_8076_4f7c_b745_f718d653e8e2">
        <rdfs:subClassOf rdf:resource="http://emmo.info/domains/emmo-units.owl#EMMO_b953f2b1_c8d1_4dd9_b630_d3ef6580c2bb"/>
        <rdfs:comment>Physical constant that by definition (after the latest revision of the SI system that was enforsed May 2019) has a known exact numerical value when expressed in SI units.</rdfs:comment>
        <rdfs:label xml:lang="en">ExactConstant</rdfs:label>
    </owl:Class>
    


    <!-- http://emmo.info/domains/emmo-physical-constants.owl#EMMO_8d689295_7d84_421b_bc01_d5cceb2c2086 -->

    <owl:Class rdf:about="http://emmo.info/domains/emmo-physical-constants.owl#EMMO_8d689295_7d84_421b_bc01_d5cceb2c2086">
        <rdfs:subClassOf rdf:resource="http://emmo.info/domains/emmo-physical-constants.owl#EMMO_3f15d200_c97b_42c8_8ac0_d81d150361e2"/>
        <rdfs:subClassOf rdf:resource="http://emmo.info/domains/emmo-units.owl#EMMO_ed4af7ae_63a2_497e_bb88_2309619ea405"/>
        <emmo-annotations:EMMO_1f1b164d_ec6a_4faa_8d5e_88bda62316cc>http://physics.nist.gov/cuu/CODATA-Value_ProtonMass</emmo-annotations:EMMO_1f1b164d_ec6a_4faa_8d5e_88bda62316cc>
        <emmo-annotations:EMMO_fe015383_afb3_44a6_ae86_043628697aa2>https://doi.org/10.1351/goldbook.P04914</emmo-annotations:EMMO_fe015383_afb3_44a6_ae86_043628697aa2>
        <rdfs:comment>The rest mass of a proton.</rdfs:comment>
        <rdfs:label xml:lang="en">ProtonMass</rdfs:label>
    </owl:Class>
    


    <!-- http://emmo.info/domains/emmo-physical-constants.owl#EMMO_99296e55_53f7_4333_9e06_760ad175a1b9 -->

    <owl:Class rdf:about="http://emmo.info/domains/emmo-physical-constants.owl#EMMO_99296e55_53f7_4333_9e06_760ad175a1b9">
        <rdfs:subClassOf rdf:resource="http://emmo.info/domains/emmo-si-units.owl#EMMO_81369540_1b0e_471b_9bae_6801af22800e"/>
        <rdfs:subClassOf rdf:resource="http://emmo.info/domains/emmo-physical-constants.owl#EMMO_89762966_8076_4f7c_b745_f718d653e8e2"/>
        <emmo-annotations:EMMO_1f1b164d_ec6a_4faa_8d5e_88bda62316cc>http://physics.nist.gov/cuu/CODATA-Value_SpeedOfLightInVacuum</emmo-annotations:EMMO_1f1b164d_ec6a_4faa_8d5e_88bda62316cc>
        <emmo-annotations:EMMO_6dd685dd_1895_46e4_b227_be9f7d643c25>http://dbpedia.org/page/Speed_of_light</emmo-annotations:EMMO_6dd685dd_1895_46e4_b227_be9f7d643c25>
        <emmo-annotations:EMMO_fe015383_afb3_44a6_ae86_043628697aa2>https://doi.org/10.1351/goldbook.S05854</emmo-annotations:EMMO_fe015383_afb3_44a6_ae86_043628697aa2>
        <rdfs:comment>The speed of light in vacuum.</rdfs:comment>
        <rdfs:label xml:lang="en">SpeedOfLightInVacuum</rdfs:label>
    </owl:Class>
    


    <!-- http://emmo.info/domains/emmo-physical-constants.owl#EMMO_a3c78d6f_ae49_47c8_a634_9b6d86b79382 -->

    <owl:Class rdf:about="http://emmo.info/domains/emmo-physical-constants.owl#EMMO_a3c78d6f_ae49_47c8_a634_9b6d86b79382">
        <rdfs:subClassOf rdf:resource="http://emmo.info/domains/emmo-physical-constants.owl#EMMO_3f15d200_c97b_42c8_8ac0_d81d150361e2"/>
        <rdfs:subClassOf rdf:resource="http://emmo.info/domains/emmo-si-units.owl#EMMO_d859588d_44dc_4614_bc75_5fcd0058acc8"/>
        <emmo-annotations:EMMO_1f1b164d_ec6a_4faa_8d5e_88bda62316cc>http://physics.nist.gov/cuu/CODATA-Value_RybergConstant</emmo-annotations:EMMO_1f1b164d_ec6a_4faa_8d5e_88bda62316cc>
        <emmo-annotations:EMMO_6dd685dd_1895_46e4_b227_be9f7d643c25>http://dbpedia.org/page/Rydberg_constant</emmo-annotations:EMMO_6dd685dd_1895_46e4_b227_be9f7d643c25>
        <emmo-annotations:EMMO_fe015383_afb3_44a6_ae86_043628697aa2>https://doi.org/10.1351/goldbook.R05430</emmo-annotations:EMMO_fe015383_afb3_44a6_ae86_043628697aa2>
        <rdfs:comment>The Rydberg constant represents the limiting value of the highest wavenumber (the inverse wavelength) of any photon that can be emitted from the hydrogen atom, or, alternatively, the wavenumber of the lowest-energy photon capable of ionizing the hydrogen atom from its ground state.</rdfs:comment>
        <rdfs:label xml:lang="en">RybergConstant</rdfs:label>
    </owl:Class>
    


    <!-- http://emmo.info/domains/emmo-physical-constants.owl#EMMO_d26baba6_1f0a_4c9f_b162_afff6ee0cd20 -->

    <owl:Class rdf:about="http://emmo.info/domains/emmo-physical-constants.owl#EMMO_d26baba6_1f0a_4c9f_b162_afff6ee0cd20">
        <rdfs:subClassOf rdf:resource="http://emmo.info/domains/emmo-physical-constants.owl#EMMO_89762966_8076_4f7c_b745_f718d653e8e2"/>
        <emmo-annotations:EMMO_1f1b164d_ec6a_4faa_8d5e_88bda62316cc>http://physics.nist.gov/cuu/CODATA-Value_JosephsonConstant</emmo-annotations:EMMO_1f1b164d_ec6a_4faa_8d5e_88bda62316cc>
        <rdfs:comment>Inverse of the magnetic flux quantum.</rdfs:comment>
        <rdfs:comment>The DBpedia definition (http://dbpedia.org/page/Magnetic_flux_quantum) is outdated as May 20, 2019. It is now an exact quantity.</rdfs:comment>
        <rdfs:label xml:lang="en">JosephsonConstant</rdfs:label>
    </owl:Class>
    


    <!-- http://emmo.info/domains/emmo-physical-constants.owl#EMMO_d7d2ca25_03e1_4099_9220_c1a58df13ad0 -->

    <owl:Class rdf:about="http://emmo.info/domains/emmo-physical-constants.owl#EMMO_d7d2ca25_03e1_4099_9220_c1a58df13ad0">
        <rdfs:subClassOf rdf:resource="http://emmo.info/domains/emmo-physical-constants.owl#EMMO_3f15d200_c97b_42c8_8ac0_d81d150361e2"/>
        <rdfs:subClassOf rdf:resource="http://emmo.info/domains/emmo-units.owl#EMMO_fdadf52c_5c39_40bc_95d9_5b7807f06e19"/>
        <emmo-annotations:EMMO_1f1b164d_ec6a_4faa_8d5e_88bda62316cc>http://physics.nist.gov/cuu/CODATA-Value_FineStructureConstant</emmo-annotations:EMMO_1f1b164d_ec6a_4faa_8d5e_88bda62316cc>
        <emmo-annotations:EMMO_6dd685dd_1895_46e4_b227_be9f7d643c25>http://dbpedia.org/page/Fine-structure_constant</emmo-annotations:EMMO_6dd685dd_1895_46e4_b227_be9f7d643c25>
        <emmo-annotations:EMMO_fe015383_afb3_44a6_ae86_043628697aa2>https://doi.org/10.1351/goldbook.F02389</emmo-annotations:EMMO_fe015383_afb3_44a6_ae86_043628697aa2>
        <rdfs:comment>A fundamental physical constant characterizing the strength of the electromagnetic interaction between elementary charged particles.</rdfs:comment>
        <rdfs:label xml:lang="en">FineStructureConstant</rdfs:label>
    </owl:Class>
    


    <!-- http://emmo.info/domains/emmo-physical-constants.owl#EMMO_da831168_975a_41f8_baae_279c298569da -->

    <owl:Class rdf:about="http://emmo.info/domains/emmo-physical-constants.owl#EMMO_da831168_975a_41f8_baae_279c298569da">
        <rdfs:subClassOf rdf:resource="http://emmo.info/domains/emmo-physical-constants.owl#EMMO_3f15d200_c97b_42c8_8ac0_d81d150361e2"/>
        <emmo-annotations:EMMO_1f1b164d_ec6a_4faa_8d5e_88bda62316cc>http://physics.nist.gov/cuu/CODATA-Value_NewtonianConstantOfGravity</emmo-annotations:EMMO_1f1b164d_ec6a_4faa_8d5e_88bda62316cc>
        <emmo-annotations:EMMO_6dd685dd_1895_46e4_b227_be9f7d643c25>http://dbpedia.org/page/Gravitational_constant</emmo-annotations:EMMO_6dd685dd_1895_46e4_b227_be9f7d643c25>
        <emmo-annotations:EMMO_fe015383_afb3_44a6_ae86_043628697aa2>https://doi.org/10.1351/goldbook.G02695</emmo-annotations:EMMO_fe015383_afb3_44a6_ae86_043628697aa2>
        <rdfs:comment>Physical constant in Newton&apos;s law of gravitation and in Einstein&apos;s general theory of relativity.</rdfs:comment>
        <rdfs:label xml:lang="en">NewtonianConstantOfGravity</rdfs:label>
    </owl:Class>
    


    <!-- http://emmo.info/domains/emmo-physical-constants.owl#EMMO_de021e4f_918f_47ef_a67b_11120f56b9d7 -->

    <owl:Class rdf:about="http://emmo.info/domains/emmo-physical-constants.owl#EMMO_de021e4f_918f_47ef_a67b_11120f56b9d7">
        <rdfs:subClassOf rdf:resource="http://emmo.info/domains/emmo-si-units.owl#EMMO_09663630_1b84_4202_91e6_e641104f579e"/>
        <rdfs:subClassOf rdf:resource="http://emmo.info/domains/emmo-physical-constants.owl#EMMO_3f15d200_c97b_42c8_8ac0_d81d150361e2"/>
        <emmo-annotations:EMMO_1f1b164d_ec6a_4faa_8d5e_88bda62316cc>http://physics.nist.gov/cuu/CODATA-Value_MagneticConstant</emmo-annotations:EMMO_1f1b164d_ec6a_4faa_8d5e_88bda62316cc>
        <rdfs:comment>The DBpedia and UIPAC Gold Book definitions (http://dbpedia.org/page/Vacuum_permeability,  https://doi.org/10.1351/goldbook.P04504) are outdated since May 20, 2019. It is now a measured constant.</rdfs:comment>
        <rdfs:comment>The value of magnetic permeability in a classical vacuum.</rdfs:comment>
        <rdfs:label xml:lang="en">VacuumMagneticPermeability</rdfs:label>
    </owl:Class>
    


    <!-- http://emmo.info/domains/emmo-physical-constants.owl#EMMO_ffc7735f_c177_46a4_98e9_a54440d29209 -->

    <owl:Class rdf:about="http://emmo.info/domains/emmo-physical-constants.owl#EMMO_ffc7735f_c177_46a4_98e9_a54440d29209">
        <rdfs:subClassOf rdf:resource="http://emmo.info/domains/emmo-physical-constants.owl#EMMO_89762966_8076_4f7c_b745_f718d653e8e2"/>
        <rdfs:subClassOf rdf:resource="http://emmo.info/domains/emmo-si-units.owl#EMMO_9bbab0be_f9cc_4f46_9f46_0fd271911b79"/>
        <emmo-annotations:EMMO_1f1b164d_ec6a_4faa_8d5e_88bda62316cc>http://physics.nist.gov/cuu/CODATA-Value_BoltzmannConstant</emmo-annotations:EMMO_1f1b164d_ec6a_4faa_8d5e_88bda62316cc>
        <emmo-annotations:EMMO_6dd685dd_1895_46e4_b227_be9f7d643c25>http://dbpedia.org/page/Boltzmann_constant</emmo-annotations:EMMO_6dd685dd_1895_46e4_b227_be9f7d643c25>
        <emmo-annotations:EMMO_fe015383_afb3_44a6_ae86_043628697aa2>https://doi.org/10.1351/goldbook.B00695</emmo-annotations:EMMO_fe015383_afb3_44a6_ae86_043628697aa2>
        <rdfs:comment>A physical constant relating energy at the individual particle level with temperature. It is the gas constant R divided by the Avogadro constant.</rdfs:comment>
        <rdfs:comment>The DBpedia definition (http://dbpedia.org/page/Boltzmann_constant) is outdated as May 20, 2019. It is now an exact quantity.</rdfs:comment>
        <rdfs:label xml:lang="en">BoltzmannConstant</rdfs:label>
    </owl:Class>
</rdf:RDF>



<!-- Generated by the OWL API (version 4.2.8.20170104-2310) https://github.com/owlcs/owlapi -->

